compiler/src/GoFlatToRiscv.v
@@ -1,0 +1,88 @@
+Require Import Coq.ZArith.BinInt.
+Require Import Coq.Lists.List. Import ListNotations.
+Require Import coqutil.Map.Interface.
+Require Import coqutil.Word.Interface coqutil.Word.Properties.
+Require Import riscv.util.Monads.
+Require Import riscv.Utility.
+Require Import riscv.Decode.
+Require Import riscv.Memory.
+Require Import riscv.Program.
+Require Import riscv.RiscvMachine.
+Require Import riscv.AxiomaticRiscv.
+Require Import riscv.Run.
+Require Import riscv.Execute.
+Require Import coqutil.Tactics.Tactics.
+Require Import compiler.containsProgram.
+Require Import compiler.FlatToRiscvBitWidthSpecifics.
+Require Import compiler.util.Tactics.
+
+Local Unset Universe Polymorphism.
+
+Section Go.
+
+  Context {W: Words}.
+  Context {RFF: RegisterFileFunctions Register word}.
+  Context {Action: Type}.
+  Context {mem: map.map word byte}.
+
+  Local Notation RiscvMachineL := (RiscvMachine Register Action).
+
+  Context {M: Type -> Type}.
+  Context {MM: Monad M}.
+  Context {RVM: RiscvProgram M word}.
+  Context {RVS: @RiscvState M word _ _ RVM}.
+  Context {RVAX: AxiomaticRiscv Action M}.
+  Context {BWS: FlatToRiscvBitWidthSpecifics word}.
+
+  Add Ring wring: (@word.ring_theory width word word_ok).
+
+  Ltac ring' := unfold ZToReg, mul, add, MkMachineWidth.MachineWidth_XLEN in *; ring.
+
+  Lemma go_left_identity{A: Type}: forall initialL post a
+         (f : A -> M unit),
+      mcomp_sat (f a) initialL post ->
+      mcomp_sat (Bind (Return a) f) initialL post.
+  Proof.
+    intros. rewrite left_identity. assumption.
+  Qed.
+
+  Lemma go_right_identity: forall initialL post
+         (m: M unit),
+      mcomp_sat m initialL post ->
+      mcomp_sat (Bind m Return) initialL post.
+  Proof.
+    intros. rewrite right_identity. assumption.
+  Qed.
+
+  Lemma go_associativity{A B: Type}: forall initialL post
+         (m: M A)
+         (f : A -> M B) (g : B -> M unit),
+      mcomp_sat (Bind m (fun x : A => Bind (f x) g)) initialL post ->
+      mcomp_sat (Bind (Bind m f) g) initialL post.
+  Proof.
+    intros. rewrite associativity. assumption.
+  Qed.
+
+  Lemma go_fetch_inst: forall {inst initialL pc0} (post: RiscvMachineL -> Prop),
+      pc0 = initialL.(getPc) ->
+      containsProgram initialL.(getMem) [inst] pc0 ->
+      mcomp_sat (Bind (execute inst) (fun _ => step)) initialL post ->
+      mcomp_sat (run1 (B := BitWidth)) initialL post.
+  Proof.
+    intros. subst.
+    unfold run1.
+    apply go_getPC.
+    unfold containsProgram in H0.
+    specialize (H0 0 _ eq_refl).
+    unfold ldInst in *.
+    destruct_one_match_hyp; [|discriminate].
+    apply invert_Some_eq_Some in H0. subst inst.
+    eapply go_loadWord; [|eassumption].
+    match goal with
+    | H: Memory.loadWord ?m ?pc = ?r |- Memory.loadWord ?m ?pc' = ?r =>
+      replace pc' with pc; [exact H|]
+    end.
+    change (4 * 0) with 0. ring'.
+  Qed.
+
+End Go.
